theories/program_logic/ectx_lifting.v
@@ -11,56 +11,56 @@ Implicit Types v : val.
 Implicit Types e : expr.
 Hint Resolve head_prim_reducible head_reducible_prim_step.
 
-Lemma wp_ectx_bind {E e} K Φ :
-  WP e @ E {{ v, WP fill K (of_val v) @ E {{ Φ }} }} ⊢ WP fill K e @ E {{ Φ }}.
+Lemma wp_ectx_bind {p E e} K Φ :
+  WP e @ p; E {{ v, WP fill K (of_val v) @ p; E {{ Φ }} }} ⊢ WP fill K e @ p; E {{ Φ }}.
 Proof. apply: weakestpre.wp_bind. Qed.
 
-Lemma wp_lift_head_step E Φ e1 :
+Lemma wp_lift_head_step p E Φ e1 :
   to_val e1 = None →
   (∀ σ1, state_interp σ1 ={E,∅}=∗
     ⌜head_reducible e1 σ1⌝ ∗
     ▷ ∀ e2 σ2 efs, ⌜head_step e1 σ1 e2 σ2 efs⌝ ={∅,E}=∗
-      state_interp σ2 ∗ WP e2 @ E {{ Φ }} ∗ [∗ list] ef ∈ efs, WP ef {{ _, True }})
-  ⊢ WP e1 @ E {{ Φ }}.
+      state_interp σ2 ∗ WP e2 @ p; E {{ Φ }} ∗ [∗ list] ef ∈ efs, WP ef @ p; ⊤ {{ _, True }})
+  ⊢ WP e1 @ p; E {{ Φ }}.
 Proof.
-  iIntros (?) "H". iApply (wp_lift_step E)=>//. iIntros (σ1) "Hσ".
+  iIntros (?) "H". iApply wp_lift_step=>//. iIntros (σ1) "Hσ".
   iMod ("H" $! σ1 with "Hσ") as "[% H]"; iModIntro.
   iSplit; first by eauto. iNext. iIntros (e2 σ2 efs) "%".
   iApply "H". by eauto.
 Qed.
 
-Lemma wp_lift_pure_head_step E Φ e1 :
+Lemma wp_lift_pure_head_step p E Φ e1 :
   (∀ σ1, head_reducible e1 σ1) →
   (∀ σ1 e2 σ2 efs, head_step e1 σ1 e2 σ2 efs → σ1 = σ2) →
   (▷ ∀ e2 efs σ, ⌜head_step e1 σ e2 σ efs⌝ →
-    WP e2 @ E {{ Φ }} ∗ [∗ list] ef ∈ efs, WP ef {{ _, True }})
-  ⊢ WP e1 @ E {{ Φ }}.
+    WP e2 @ p; E {{ Φ }} ∗ [∗ list] ef ∈ efs, WP ef @ p; ⊤ {{ _, True }})
+  ⊢ WP e1 @ p; E {{ Φ }}.
 Proof.
   iIntros (??) "H". iApply wp_lift_pure_step; eauto. iNext.
   iIntros (????). iApply "H". eauto.
 Qed.
 
-Lemma wp_lift_atomic_head_step {E Φ} e1 :
+Lemma wp_lift_atomic_head_step {p E Φ} e1 :
   to_val e1 = None →
   (∀ σ1, state_interp σ1 ={E}=∗
     ⌜head_reducible e1 σ1⌝ ∗
     ▷ ∀ e2 σ2 efs, ⌜head_step e1 σ1 e2 σ2 efs⌝ ={E}=∗
       state_interp σ2 ∗
-      default False (to_val e2) Φ ∗ [∗ list] ef ∈ efs, WP ef {{ _, True }})
-  ⊢ WP e1 @ E {{ Φ }}.
+      default False (to_val e2) Φ ∗ [∗ list] ef ∈ efs, WP ef @ p; ⊤ {{ _, True }})
+  ⊢ WP e1 @ p; E {{ Φ }}.
 Proof.
   iIntros (?) "H". iApply wp_lift_atomic_step; eauto.
   iIntros (σ1) "Hσ1". iMod ("H" $! σ1 with "Hσ1") as "[% H]"; iModIntro.
   iSplit; first by eauto. iNext. iIntros (e2 σ2 efs) "%". iApply "H"; auto.
 Qed.
 
-Lemma wp_lift_atomic_head_step_no_fork {E Φ} e1 :
+Lemma wp_lift_atomic_head_step_no_fork {p E Φ} e1 :
   to_val e1 = None →
   (∀ σ1, state_interp σ1 ={E}=∗
     ⌜head_reducible e1 σ1⌝ ∗
     ▷ ∀ e2 σ2 efs, ⌜head_step e1 σ1 e2 σ2 efs⌝ ={E}=∗
       ⌜efs = []⌝ ∗ state_interp σ2 ∗ default False (to_val e2) Φ)
-  ⊢ WP e1 @ E {{ Φ }}.
+  ⊢ WP e1 @ p; E {{ Φ }}.
 Proof.
   iIntros (?) "H". iApply wp_lift_atomic_head_step; eauto.
   iIntros (σ1) "Hσ1". iMod ("H" $! σ1 with "Hσ1") as "[$ H]"; iModIntro.
@@ -69,20 +69,20 @@ Proof.
   by iApply big_sepL_nil.
 Qed.
 
-Lemma wp_lift_pure_det_head_step {E Φ} e1 e2 efs :
+Lemma wp_lift_pure_det_head_step {p E Φ} e1 e2 efs :
   (∀ σ1, head_reducible e1 σ1) →
   (∀ σ1 e2' σ2 efs',
     head_step e1 σ1 e2' σ2 efs' → σ1 = σ2 ∧ e2 = e2' ∧ efs = efs') →
-  ▷ (WP e2 @ E {{ Φ }} ∗ [∗ list] ef ∈ efs, WP ef {{ _, True }})
-  ⊢ WP e1 @ E {{ Φ }}.
+  ▷ (WP e2 @ p; E {{ Φ }} ∗ [∗ list] ef ∈ efs, WP ef @ p; ⊤ {{ _, True }})
+  ⊢ WP e1 @ p; E {{ Φ }}.
 Proof. eauto using wp_lift_pure_det_step. Qed.
 
-Lemma wp_lift_pure_det_head_step_no_fork {E Φ} e1 e2 :
+Lemma wp_lift_pure_det_head_step_no_fork {p E Φ} e1 e2 :
   to_val e1 = None →
   (∀ σ1, head_reducible e1 σ1) →
   (∀ σ1 e2' σ2 efs',
     head_step e1 σ1 e2' σ2 efs' → σ1 = σ2 ∧ e2 = e2' ∧ [] = efs') →
-  ▷ WP e2 @ E {{ Φ }} ⊢ WP e1 @ E {{ Φ }}.
+  ▷ WP e2 @ p; E {{ Φ }} ⊢ WP e1 @ p; E {{ Φ }}.
 Proof.
   intros. rewrite -(wp_lift_pure_det_step e1 e2 []) ?big_sepL_nil ?right_id; eauto.
 Qed.
